Lithium and performance experiments

src/Iris/Examples/IRun.lean
@@ -38,15 +38,43 @@ partial def irunCore (nsteps : Option Nat) : TacticM Unit := do profileitM Excep
   let mut n := 0
   let mut shelved := []
   repeat
-    if nsteps = some n then
+    if nsteps == some n then
       break
-    let goal::goals' := goals | break
+    let mut goal::goals' := goals | break
     if ← goal.isAssigned then
       goals := goals'
       continue
-    let (progress, goals', shelved') ← goal.withContext do
+    -- reduce matches
+    let mut progress_match := false
+
+    repeat do
       let g ← instantiateMVars <| ← goal.getType
+      let some #[prop, bi, P, G] := g.appM? ``Entails' | throwError "not in proof mode"
+      unless (← isMatcherApp G) do
+        break
+      match (← reduceRecMatcher? G) with
+      | some G' =>
+        let g' := mkApp4 (.const ``Entails' [g.getAppFn.constLevels![0]!])
+          prop bi P G'
+        goal := ← goal.replaceTargetDefEq g'
+        progress_match := true
+        -- logInfo m!"AFTER REDUCE: {← goal.getType}"
+      | none    => throwError s!"Cannot reduce matcher at step {n}"
+
+/-
+    let ext ← Lean.Meta.getSimpExtension? `irun_simp
+    let theorems ← ext.get!.getTheorems
+    let { ctx:=simpctx, .. } ← goal.withContext <| mkSimpContext .missing (eraseLocal := false) (kind := .dsimp) (simpTheorems := pure theorems)
+    let g ← instantiateMVars <| ← goal.getType
+    let ⟨g_new, _⟩ ← Meta.dsimp g simpctx {}
+    goal := ← goal.replaceTargetDefEq g_new
+-/
+
+    -- find a tactic or lemma to apply to the goal
+    let (progress, goals'', shelved') ← goal.withContext do
+      let mut g ← instantiateMVars <| ← goal.getType
       let some { u, prop, bi, e, hyps, goal:=G } := parseIrisGoal? g | throwError "not in proof mode"
+      -- logInfo m!"IN LOOP: {G}"
       let tree := irunExt.getState (← getEnv)
       let G ← instantiateExprMVars G
       if G.isMVar then throwError "irun failed: goal has free metavars"
@@ -60,7 +88,13 @@ partial def irunCore (nsteps : Option Nat) : TacticM Unit := do profileitM Excep
           let (args, _, targetTy) ← forallMetaTelescopeReducing (← inferType pf)
           let .some (Gnew, Gdecl) := (unpackEntails targetTy) | throwError "theorem is not entails, this should not happen"
           let .true ← isDefEq G Gdecl | continue
-          -- TODO: try to solve all unsolved args using a tactic
+
+          for mvar in args do
+            let mvarId := mvar.mvarId!
+            if ! (← mvarId.isAssigned) && ! (← mvarId.isDelayedAssigned) then
+              -- TODO: try to solve all unsolved args using a tactic
+              throwError s!"not assigned: {← mvarId.getType}"
+
           let m ← mkFreshExprSyntheticOpaqueMVar <|
             IrisGoal.toExpr { prop, bi, hyps := hyps, goal := Gnew }
           let pf := mkApp7 (.const ``irun_apply [u]) prop bi e G Gnew (mkAppN pf args) m
@@ -71,13 +105,13 @@ partial def irunCore (nsteps : Option Nat) : TacticM Unit := do profileitM Excep
           return (true, goals_new++goals', shelved++shelved_new)
       return (false, goal::goals', shelved)
       --return (true, goal::goals', shelved)
-    if !progress then
+    if !progress && !progress_match then
       break
     n := n+1
-    goals := goals'
+    goals := goals''
     shelved := shelved'
 
-  if !(nsteps = .none || nsteps = .some n) then
+  if !(nsteps == .none || nsteps == .some n) then
     logInfo s!"Did {n} steps"
   setGoals (goals ++ shelved)
 
@@ -136,345 +170,5 @@ elab "irun" colGt nsteps:num : tactic => do
   irunCore (some nsteps.getNat)
 
 elab "irun" colGt "∞" : tactic => do
+  -- this number is sufficiently close to infinity for our purposes
   irunCore (some 100000)
-
-@[irun]
-theorem li_assoc_star.{u} {PROP : Type u} [BI PROP] {P1 P2 P3 : PROP}
- : P1 ∗ (P2 ∗ P3) ⊢ (P1 ∗ P2) ∗ P3 :=
-   sorry
-
-axiom PROPTest : Type
-axiom BIPROPTest : BI PROPTest
-noncomputable instance BIPROPTest_inst : BI PROPTest := BIPROPTest
-
-noncomputable def PROPTest_test : PROPTest := iprop(True)
-
-def prop_test [BI PROP] : PROP := iprop(True)
-
-@[irun_tac 100 | PROPTest_test, iprop((∃ _, ∀ _, prop_test ∗ _)), iprop((⌜_⌝ ∗ _ ∗ _) -∗ _), _ ∗ _]
-def irunTest : IRunTacticType := fun goal => do
-  IO.println s!"Test Tac {← ppExpr (← goal.getType)}"
-  return none
-
-
-theorem intro_tac [BI PROP] {P A Q : PROP}
-  (h : P ∗ A ⊢ Q)
- : P ⊢ A -∗ Q := wand_intro h
-
-@[irun_tac _ -∗ _]
-def irunIntro : IRunTacticType := fun goal => do profileitM Exception "irunIntro" (← getOptions) do
-  let g ← instantiateMVars <| ← goal.getType
-  let some { prop, bi, e, hyps, goal:=G } := parseIrisGoal? g | throwError "not in proof mode"
-  let ~q(iprop($A -∗ $Q)) := G | return none
-  let ident ← `(binderIdent| _)
-  let (b, A') := if A.isAppOfArity ``intuitionistically 3 then
-      (q(true), A.getArg! 3)
-    else
-      (q(false), A)
-  let goals ← IO.mkRef #[]
-  let pf ← iCasesCore bi hyps Q b A A' ⟨⟩ (.one ident) fun hyps => do
-    let m ← mkFreshExprSyntheticOpaqueMVar <|
-      IrisGoal.toExpr { prop, bi, hyps, goal:=Q }
-    goals.modify (·.push m.mvarId!)
-    return m
-  let pf := q(@intro_tac $prop $bi $e $A $Q $pf)
-  goal.assign pf
-  return .some ((← goals.get).toList, [])
-
-theorem cancel [BI PROP] {p : Bool} {P P' A Q' : PROP}
-  (hP : P ⊣⊢ P' ∗ □?p A)
-  (h : P' ⊢ Q')
- : P ⊢ A ∗ Q' :=
-   hP.1.trans <| sep_comm.1.trans <| sep_mono intuitionisticallyIf_elim h
-
-@[irun_tac _ ∗ _]
-def irunCancel : IRunTacticType := fun goal => do profileitM Exception "irunCancel" (← getOptions) do
-  let g ← instantiateMVars <| ← goal.getType
-  let some { prop, bi, hyps, goal:=G } := parseIrisGoal? g | throwError "not in proof mode"
-  let ~q(iprop($A ∗ $Q)) := G | return none
-  let some ⟨_inst, P', hyps, out, ty, b, _, pf⟩ ←
-    hyps.removeG false fun _ _ _ ty => do
-      -- logInfo m!"ty: ${ty}, A: ${A}"
-      if ← isDefEq ty A then return some ty else return none
-    | return none
-  have : $ty =Q $A := ⟨⟩
-  have : $out =Q iprop(□?$b $ty) := ⟨⟩
-  let m : Q($P' ⊢ $Q) ← mkFreshExprSyntheticOpaqueMVar <|
-    IrisGoal.toExpr { prop, bi, hyps := hyps, goal := Q }
-  let pf := q(cancel $pf $m)
-  goal.assign pf
-  return .some ([m.mvarId!], [])
-
-theorem true_tac [BI PROP] (P : PROP)
- : P ⊢ True := pure_intro .intro
-
-@[irun_tac True]
-def irunTrue : IRunTacticType := fun goal => do profileitM Exception "irunTrue" (← getOptions) do
-  let g ← instantiateMVars <| ← goal.getType
-  let some { prop:=prop, bi:=bi, hyps:=_, e, goal:=G } := parseIrisGoal? g | throwError "not in proof mode"
-  let ~q(iprop(True)) := G | return none
-  let pf := q(@true_tac $prop $bi $e)
-  goal.assign pf
-  return .some ([], [])
-
-section test
-variable {u} [BI.{u} PROP]
-theorem proof_test (P : Nat → PROP) (Q : PROP) :
-  ⊢ Q -∗ P 1 -∗ P 2 -∗ ⌜1=1⌝ -∗ (P 1 ∗ P 2) ∗ Q ∗ True
-:= by
-  istart
-  irun
-end test
-
-def lif [BI PROP] (cond : Prop) (P1 P2 : PROP) : PROP :=
-  iprop((⌜cond⌝ -∗ P1) ∧ (⌜¬cond⌝ -∗ P2))
-
-theorem lif_true [BI PROP] {cond} {P P1 P2 : PROP}
-  (h1 : cond)
-  (h2 : P ⊢ P1)
- : P ⊢ lif cond P1 P2 :=
-   sorry
-
-theorem lif_false [BI PROP] {cond} {P P1 P2 : PROP}
-  (h1 : ¬ cond)
-  (h2 : P ⊢ P2)
- : P ⊢ lif cond P1 P2 :=
-   sorry
-
-syntax "istepsolve" : tactic
---macro_rules
---  | `(tactic|istepsolve) => `(tactic|trivial)
-macro_rules
-  | `(tactic|istepsolve) => `(tactic|solve| simp)
-
-@[irun_tac lif _ _ _]
-def irunLif : IRunTacticType := fun goal => do profileitM Exception "irunLif" (← getOptions) do
-  let g ← instantiateMVars <| ← goal.getType
-  let some { prop, bi, e, hyps, goal:=G } := parseIrisGoal? g | throwError "not in proof mode"
-  let ~q(iprop(lif $cond $P1 $P2)) := G | return none
-
-  let mcond : Q($cond) ← mkFreshExprSyntheticOpaqueMVar cond
-  try
-    let _ ← evalTacticAtRaw (← `(tactic|istepsolve)) mcond.mvarId!
-    let m : Q($e ⊢ $P1) ← mkFreshExprSyntheticOpaqueMVar <|
-      IrisGoal.toExpr { prop, bi, hyps := hyps, goal := P1 }
-    let pf := q(lif_true (P2:=$P2) $mcond $m)
-    goal.assign pf
-    return .some ([m.mvarId!], [])
-  catch _ => pure ()
-
-  let mnegcond : Q(¬$cond) ← mkFreshExprSyntheticOpaqueMVar q(¬ $cond)
-  try
-    let _ ← evalTacticAt (← `(tactic|istepsolve)) mnegcond.mvarId!
-    let m : Q($e ⊢ $P2) ← mkFreshExprSyntheticOpaqueMVar <|
-      IrisGoal.toExpr { prop, bi, hyps := hyps, goal := P2 }
-    let pf := q(lif_false (P1:=$P1) $mnegcond $m)
-    goal.assign pf
-    return .some ([m.mvarId!], [])
-  catch _ => pure ()
-
-  throwError "Cannot solve either side of lif"
-
-end Iris.ProofMode
-
-namespace Iris.Examples
-open Iris.BI
-
-section lang
-variable {u} [BI.{u} PROP]
-def Loc : Type := Nat
-
-inductive Binop where
-| plus | minus | eq
-
-mutual
-inductive Val where
-| nat : Nat -> Val
-| loc : Loc -> Val
-| recv : String -> String -> Expr -> Val
-inductive Expr where
-| val : Val -> Expr
-| var : String -> Expr
-| binop : Expr -> Binop -> Expr -> Expr
-| rece : String -> String -> Expr -> Expr
-| app : Expr -> Expr -> Expr
-| ife : Expr -> Expr -> Expr -> Expr
-end
-
-def subst (x : String) (v : Val) (e : Expr) : Expr :=
-  match e with
-  | .val _ => e
-  | .var y => if x = y then .val v else e
-  | .binop e1 o e2 => .binop (subst x v e1) o (subst x v e2)
-  | .rece f y e' => .rece f y (if x = f || x = y then e' else subst x v e')
-  | .app e1 e2 => .app (subst x v e1) (subst x v e2)
-  | .ife e1 e2 e3 => .ife (subst x v e1) (subst x v e2)  (subst x v e3)
-
-def wp [BI PROP] (e : Expr) (P : Val -> PROP) : PROP := by sorry
-def wpnat (v : Val) (P : Nat -> PROP) : PROP := iprop(∃ n, ⌜v = .nat n⌝ ∗ P n)
-def wprecv (v : Val) (P : String -> String -> Expr -> PROP) : PROP := iprop(∃ f x e, ⌜v = .recv f x e⌝ ∗ P f x e)
-def wpsubst (x : String) (v : Val) (e : Expr) (P : Expr -> PROP) : PROP := P (subst x v e)
-
-@[irun]
-theorem wpnat_nat (n : Nat) (P : Nat -> PROP) : P n ⊢ wpnat (.nat n) P := by
-  unfold wpnat
-  iintro HP
-  iexists _
-  isplit
-  · ipure_intro
-    rfl
-  · iassumption
-
-@[irun]
-theorem wprecv_rec f x e (P : String -> String -> Expr -> PROP) : P f x e ⊢ wprecv (.recv f x e) P := by
-  unfold wprecv
-  iintro HP
-  iexists _
-  iexists _
-  iexists _
-  isplit
-  · ipure_intro
-    rfl
-  · iassumption
-
-@[irun]
- theorem wp_val v (P : Val -> PROP) :
-  P v ⊢ wp (.val v) P := by sorry
-
-@[irun]
-theorem wp_plus e1 e2 (P : Val -> PROP) :
-  (wp e1 λ v1 =>
-   wp e2 λ v2 =>
-   wpnat v1 λ n1 =>
-   wpnat v2 λ n2 =>
-   P (.nat (n1 + n2))) ⊢ wp (Expr.binop e1 .plus e2) P := by sorry
-
-@[irun]
-theorem wp_minus e1 e2 (P : Val -> PROP) :
-  (wp e1 λ v1 =>
-   wp e2 λ v2 =>
-   wpnat v1 λ n1 =>
-   wpnat v2 λ n2 =>
-   P (.nat (n1 - n2))) ⊢ wp (Expr.binop e1 .minus e2) P := by sorry
-
-@[irun]
-theorem wp_eq e1 e2 (P : Val -> PROP) :
-  (wp e1 λ v1 =>
-   wp e2 λ v2 =>
-   wpnat v1 λ n1 =>
-   wpnat v2 λ n2 =>
-   P (.nat (if n1 = n2 then 1 else 0))) ⊢ wp (Expr.binop e1 .eq e2) P := by sorry
-
-@[irun]
-theorem wp_rec (P : Val -> PROP) :
-  (P (.recv f x e)) ⊢ wp (.rece f x e) P := by sorry
-
-@[irun]
-theorem wp_app e1 e2 (P : Val -> PROP) :
-  (wp e2 λ v2 =>
-   wp e1 λ v1 =>
-   wprecv v1 λ f x e' =>
-   wpsubst x v2 e' λ e =>
-   wpsubst f (.recv f x e') e λ e =>
-   wp e P) ⊢ wp (.app e1 e2) P := by sorry
-
-@[irun]
-theorem wp_if e1 e2 e3 (P : Val -> PROP) :
-  (wp e1 λ v1 =>
-   wpnat v1 λ n1 =>
-   ProofMode.lif (n1 ≠ 0) (wp e2 P) (wp e3 P)) ⊢
-  wp (.ife e1 e2 e3) P := by sorry
-
-
-section
-open Lean Elab Tactic Meta Qq BI Std ProofMode
-@[irun_tac wpsubst _ _ _ _]
-def irunSubst : IRunTacticType := fun goal => do profileitM Exception "irunSubst" (← getOptions) do
-  let g ← instantiateMVars <| ← goal.getType
-  let some { prop:=_, bi:=_, e:=_, hyps:=_, goal:=G } := parseIrisGoal? g | throwError "not in proof mode"
-
-  let .true := G.isAppOfArity ``wpsubst 5 | return none
-  -- TODO: Do something smarter here?
-  let goals ← evalTacticAtRaw (← `(tactic | dsimp [wpsubst, subst])) goal
-  return .some (goals, [])
-
-end
-end lang
-
-theorem exfalso {P : Prop} : P  :=
-  by sorry
-
-section
-variable {u} [BI.{u} PROP]
-
-theorem proof_intro_custom_auto (P G : PROP) :
-  ⊢ P -∗ G -∗ G ∗ True := by
-    istart
-    irun
-
-theorem proof_intro_pers_auto (P G : PROP) :
-  ⊢ P -∗ □ G -∗ G ∗ G ∗ True := by
-    istart
-    irun
-
---set_option profiler true in
-#time theorem proof_intro_2 [BIAffine PROP] (P : Nat → PROP) :
-  ⊢ List.foldl (λ G n => iprop((P n) -∗ G)) (P 119) (List.range 120)
-:=
-  -- set_option trace.profiler true in by
-   by
-     dsimp [List.foldl, List.range, List.range.loop] <;> (repeat iintro _) <;> iassumption
-
-
--- TODO: why does ilif sometimes take more than 1ms here if there a no lif in the goal?
---set_option profiler true in
---set_option profiler.threshold 1 in
-set_option maxRecDepth 30000 in
-#time theorem proof_cancel_2 (P : Nat → PROP) :
-  ⊢ List.foldl (λ G n => iprop((P n) -∗ G))
-    (List.foldl (λ G n => iprop(P n ∗ G)) iprop(True) (
-    -- List.reverse makes cancellation basically instant
-    -- List.reverse
-    (List.range 100)))
-    (List.range 100)
-:=
-  by
-    dsimp [List.foldl, List.range, List.range.loop, List.reverse]
-    istart
-    -- set_option trace.profiler true in
-    -- set_option trace.profiler.threshold 1 in
-    irun
-
-theorem wp_test (P : Val -> PROP) :
-  P (.nat 10) ⊢ wp (Expr.binop (.val (.nat 5)) .plus (.val (.nat 5))) (λ v => iprop(P v ∗ True)) := by
-  istart
-  irun 1
-  irun 1
-  irun 1
-  irun 1
-  irun 1
-  irun 1
-  irun 1
-  irun 1
-
-def rec_fn : Val :=
-  .recv "f" "x" (.ife (.binop (.var "x") .eq (.val (.nat 0))) (.val (.nat 0)) (.app (.var "f") (.binop (.var "x") .minus (.val (.nat 1)))))
-
---set_option profiler true in
---set_option profiler.threshold 1 in
-#time theorem wp_test2 (P : Val -> PROP) :
-  P (.nat 0) ⊢ wp (.app (.val rec_fn) (.val (.nat 100))) (λ v => iprop(P v ∗ True)) := by
-  istart
-  unfold rec_fn
-  --isubst <;> iautoapply
-  --set_option trace.profiler true in
-  --set_option trace.profiler.threshold 1 in
-  --set_option diagnostics true in
-  --set_option profiler true in
-  irun ∞
-  -- rep 300 istep
-  --repeat' istep
-
-end
-
-end Iris.Examples
