src/Iris/Examples/IRunTest.lean
@@ -1,0 +1,474 @@
+/-
+Copyright (c) 2025 Michael Sammler. All rights reserved.
+Released under Apache 2.0 license as described in the file LICENSE.
+Authors: Michael Sammler
+-/
+import Iris.BI
+import Iris.ProofMode
+import Iris.Examples.IRunAttr
+import Iris.Examples.IRun
+
+
+namespace Iris.ProofMode
+open Lean Elab Tactic Meta Qq BI Std
+
+@[irun]
+theorem li_assoc_star.{u} {PROP : Type u} [BI PROP] {P1 P2 P3 : PROP}
+ : P1 ∗ (P2 ∗ P3) ⊢ (P1 ∗ P2) ∗ P3 :=
+   sorry
+
+axiom PROPTest : Type
+axiom BIPROPTest : BI PROPTest
+noncomputable instance BIPROPTest_inst : BI PROPTest := BIPROPTest
+
+noncomputable def PROPTest_test : PROPTest := iprop(True)
+
+def prop_test [BI PROP] : PROP := iprop(True)
+
+@[irun_tac 100 | PROPTest_test, iprop((∃ _, ∀ _, prop_test ∗ _)), iprop((⌜_⌝ ∗ _ ∗ _) -∗ _), _ ∗ _]
+def irunTest : IRunTacticType := fun goal => do
+  IO.println s!"Test Tac {← ppExpr (← goal.getType)}"
+  return none
+
+
+theorem intro_tac [BI PROP] {P A Q : PROP}
+  (h : P ∗ A ⊢ Q)
+ : P ⊢ A -∗ Q := wand_intro h
+
+@[irun_tac _ -∗ _]
+def irunIntro : IRunTacticType := fun goal => do profileitM Exception "irunIntro" (← getOptions) do
+  let g ← instantiateMVars <| ← goal.getType
+  let some { prop, bi, e, hyps, goal:=G } := parseIrisGoal? g | throwError "not in proof mode"
+  let ~q(iprop($A -∗ $Q)) := G | return none
+  let ident ← `(binderIdent| _)
+  let (b, A') := if A.isAppOfArity ``intuitionistically 3 then
+      (q(true), A.getArg! 3)
+    else
+      (q(false), A)
+  let goals ← IO.mkRef #[]
+  let pf ← iCasesCore bi hyps Q b A A' ⟨⟩ (.one ident) fun hyps => do
+    let m ← mkFreshExprSyntheticOpaqueMVar <|
+      IrisGoal.toExpr { prop, bi, hyps, goal:=Q }
+    goals.modify (·.push m.mvarId!)
+    return m
+  let pf := q(@intro_tac $prop $bi $e $A $Q $pf)
+  goal.assign pf
+  return .some ((← goals.get).toList, [])
+
+theorem cancel [BI PROP] {p : Bool} {P P' A Q' : PROP}
+  (hP : P ⊣⊢ P' ∗ □?p A)
+  (h : P' ⊢ Q')
+ : P ⊢ A ∗ Q' :=
+   hP.1.trans <| sep_comm.1.trans <| sep_mono intuitionisticallyIf_elim h
+
+@[irun_tac _ ∗ _]
+def irunCancel : IRunTacticType := fun goal => do profileitM Exception "irunCancel" (← getOptions) do
+  let g ← instantiateMVars <| ← goal.getType
+  let some { prop, bi, hyps, goal:=G } := parseIrisGoal? g | throwError "not in proof mode"
+  let ~q(iprop($A ∗ $Q)) := G | return none
+  let some ⟨_inst, P', hyps, out, ty, b, _, pf⟩ ←
+    hyps.removeG false fun _ _ _ ty => do
+      -- logInfo m!"ty: ${ty}, A: ${A}"
+      if ← isDefEq ty A then return some ty else return none
+    | return none
+  have : $ty =Q $A := ⟨⟩
+  have : $out =Q iprop(□?$b $ty) := ⟨⟩
+  let m : Q($P' ⊢ $Q) ← mkFreshExprSyntheticOpaqueMVar <|
+    IrisGoal.toExpr { prop, bi, hyps := hyps, goal := Q }
+  let pf := q(cancel $pf $m)
+  goal.assign pf
+  return .some ([m.mvarId!], [])
+
+theorem true_tac [BI PROP] (P : PROP)
+ : P ⊢ True := pure_intro .intro
+
+@[irun_tac True]
+def irunTrue : IRunTacticType := fun goal => do profileitM Exception "irunTrue" (← getOptions) do
+  let g ← instantiateMVars <| ← goal.getType
+  let some { prop:=prop, bi:=bi, hyps:=_, e, goal:=G } := parseIrisGoal? g | throwError "not in proof mode"
+  let ~q(iprop(True)) := G | return none
+  let pf := q(@true_tac $prop $bi $e)
+  goal.assign pf
+  return .some ([], [])
+
+section test
+variable {u} [BI.{u} PROP]
+theorem proof_test (P : Nat → PROP) (Q : PROP) :
+  ⊢ Q -∗ P 1 -∗ P 2 -∗ ⌜1=1⌝ -∗ (P 1 ∗ P 2) ∗ Q ∗ True
+:= by
+  istart
+  irun ∞
+end test
+
+def lif [BI PROP] (cond : Prop) (P1 P2 : PROP) : PROP :=
+  iprop((⌜cond⌝ -∗ P1) ∧ (⌜¬cond⌝ -∗ P2))
+
+theorem lif_true [BI PROP] {cond} {P P1 P2 : PROP}
+  (h1 : cond)
+  (h2 : P ⊢ P1)
+ : P ⊢ lif cond P1 P2 :=
+   sorry
+
+theorem lif_false [BI PROP] {cond} {P P1 P2 : PROP}
+  (h1 : ¬ cond)
+  (h2 : P ⊢ P2)
+ : P ⊢ lif cond P1 P2 :=
+   sorry
+
+syntax "istepsolve" : tactic
+--macro_rules
+--  | `(tactic|istepsolve) => `(tactic|trivial)
+macro_rules
+  | `(tactic|istepsolve) => `(tactic|solve| simp)
+
+@[irun_tac lif _ _ _]
+def irunLif : IRunTacticType := fun goal => do profileitM Exception "irunLif" (← getOptions) do
+  let g ← instantiateMVars <| ← goal.getType
+  let some { prop, bi, e, hyps, goal:=G } := parseIrisGoal? g | throwError "not in proof mode"
+  let ~q(iprop(lif $cond $P1 $P2)) := G | return none
+
+  let mcond : Q($cond) ← mkFreshExprSyntheticOpaqueMVar cond
+  try
+    let _ ← evalTacticAtRaw (← `(tactic|istepsolve)) mcond.mvarId!
+    let m : Q($e ⊢ $P1) ← mkFreshExprSyntheticOpaqueMVar <|
+      IrisGoal.toExpr { prop, bi, hyps := hyps, goal := P1 }
+    let pf := q(lif_true (P2:=$P2) $mcond $m)
+    goal.assign pf
+    return .some ([m.mvarId!], [])
+  catch _ => pure ()
+
+  let mnegcond : Q(¬$cond) ← mkFreshExprSyntheticOpaqueMVar q(¬ $cond)
+  try
+    let _ ← evalTacticAt (← `(tactic|istepsolve)) mnegcond.mvarId!
+    let m : Q($e ⊢ $P2) ← mkFreshExprSyntheticOpaqueMVar <|
+      IrisGoal.toExpr { prop, bi, hyps := hyps, goal := P2 }
+    let pf := q(lif_false (P1:=$P1) $mnegcond $m)
+    goal.assign pf
+    return .some ([m.mvarId!], [])
+  catch _ => pure ()
+
+  throwError "Cannot solve either side of lif"
+
+end Iris.ProofMode
+
+namespace Iris.Examples
+open BI
+
+section lang
+variable {u} [BI.{u} PROP]
+def Loc : Type := Nat
+
+inductive Binop where
+| plus | minus | eq
+
+mutual
+inductive Val where
+| nat : Nat -> Val
+| loc : Loc -> Val
+| recv : String -> String -> Exp -> Val
+inductive Exp where
+| val : Val -> Exp
+| var : String -> Exp
+| binop : Exp -> Binop -> Exp -> Exp
+| rece : String -> String -> Exp -> Exp
+| app : Exp -> Exp -> Exp
+| ife : Exp -> Exp -> Exp -> Exp
+end
+
+def subst (x : String) (v : Val) (e : Exp) : Exp :=
+  match e with
+  | .val _ => e
+  | .var y => if x == y then .val v else e
+  | .binop e1 o e2 => .binop (subst x v e1) o (subst x v e2)
+  | .rece f y e' => .rece f y (if x == f || x == y then e' else subst x v e')
+  | .app e1 e2 => .app (subst x v e1) (subst x v e2)
+  | .ife e1 e2 e3 => .ife (subst x v e1) (subst x v e2)  (subst x v e3)
+
+def wp [BI PROP] (e : Exp) (P : Val -> PROP) : PROP := by sorry
+def wpnat (v : Val) (P : Nat -> PROP) : PROP := iprop(∃ n, ⌜v = .nat n⌝ ∗ P n)
+def wprecv (v : Val) (P : String -> String -> Exp -> PROP) : PROP := iprop(∃ f x e, ⌜v = .recv f x e⌝ ∗ P f x e)
+def wpsubst (x : String) (v : Val) (e : Exp) (P : Exp -> PROP) : PROP := P (subst x v e)
+
+def wpsimp {α : Type _} [BI PROP] (_ : Lean.Name) (a : α) (P : α -> PROP) : PROP := P a
+
+@[irun]
+theorem wpnat_nat (n : Nat) (P : Nat -> PROP) : P n ⊢ wpnat (.nat n) P := by
+  unfold wpnat
+  iintro HP
+  iexists _
+  isplit
+  · ipure_intro
+    rfl
+  · iassumption
+
+@[irun]
+theorem wprecv_rec f x e (P : String -> String -> Exp -> PROP) : P f x e ⊢ wprecv (.recv f x e) P := by
+  unfold wprecv
+  iintro HP
+  iexists _
+  iexists _
+  iexists _
+  isplit
+  · ipure_intro
+    rfl
+  · iassumption
+
+@[irun]
+ theorem wp_val v (P : Val -> PROP) :
+  P v ⊢ wp (.val v) P := by sorry
+
+@[irun]
+theorem wp_plus e1 e2 (P : Val -> PROP) :
+  (wp e1 λ v1 =>
+   wp e2 λ v2 =>
+   wpnat v1 λ n1 =>
+   wpnat v2 λ n2 =>
+   wpsimp `irun_simp (n1 + n2) λ n =>
+   P (.nat n)) ⊢ wp (Exp.binop e1 .plus e2) P := by sorry
+
+@[irun]
+theorem wp_minus e1 e2 (P : Val -> PROP) :
+  (wp e1 λ v1 =>
+   wp e2 λ v2 =>
+   wpnat v1 λ n1 =>
+   wpnat v2 λ n2 =>
+   wpsimp `irun_simp (n1 - n2) λ n =>
+   P (.nat n)) ⊢ wp (Exp.binop e1 .minus e2) P := by sorry
+
+@[irun]
+theorem wp_eq e1 e2 (P : Val -> PROP) :
+  (wp e1 λ v1 =>
+   wp e2 λ v2 =>
+   wpnat v1 λ n1 =>
+   wpnat v2 λ n2 =>
+   wpsimp `irun_simp (if n1 == n2 then 1 else 0) λ n =>
+   P (.nat n)) ⊢ wp (Exp.binop e1 .eq e2) P := by sorry
+
+@[irun]
+theorem wp_rec (P : Val -> PROP) :
+  (P (.recv f x e)) ⊢ wp (.rece f x e) P := by sorry
+
+@[irun]
+theorem wp_app e1 e2 (P : Val -> PROP) :
+  (wp e2 λ v2 =>
+   wp e1 λ v1 =>
+   wprecv v1 λ f x e' =>
+   wpsubst x v2 e' λ e =>
+   wpsubst f (.recv f x e') e λ e =>
+   wp e P) ⊢ wp (.app e1 e2) P := by sorry
+
+@[irun]
+theorem wp_if e1 e2 e3 (P : Val -> PROP) :
+  (wp e1 λ v1 =>
+   wpnat v1 λ n1 =>
+   ProofMode.lif (n1 ≠ 0) (wp e2 P) (wp e3 P)) ⊢
+  wp (.ife e1 e2 e3) P := by sorry
+
+namespace Reify
+open Lean
+inductive Exp where
+| val : Expr -> Exp -- we do not need to reify values
+| var : String -> Exp
+| binop : Exp -> Expr -> Exp -> Exp
+| rece : String -> String -> Exp -> Exp
+| app : Exp -> Exp -> Exp
+| ife : Exp -> Exp -> Exp -> Exp
+| unk : Expr -> Exp
+deriving Inhabited, Repr
+
+-- should this be ToExpr?
+def Exp.unreify : Exp → Expr
+  | .val v => mkApp (mkConst ``Examples.Exp.val) v
+  | .var v => mkApp (mkConst ``Examples.Exp.var) (mkStrLit v)
+  | .binop e1 o e2 => mkApp3 (mkConst ``Examples.Exp.binop) (unreify e1) o (unreify e2)
+  | .rece f x e => mkApp3 (mkConst ``Examples.Exp.rece) (mkStrLit f) (mkStrLit x) (unreify e)
+  | .app e1 e2 => mkApp2 (mkConst ``Examples.Exp.app) (unreify e1) (unreify e2)
+  | .ife e1 e2 e3 => mkApp3 (mkConst ``Examples.Exp.ife) (unreify e1) (unreify e2) (unreify e3)
+  | .unk e => e
+
+
+def rawStringLit? : Expr → Option String
+  | .lit (.strVal v) => .some v
+  | _ => .none
+
+
+partial def reify (e : Expr) : Exp :=
+  match_expr e with
+  | Examples.Exp.val v => .val v
+  | Examples.Exp.var v =>
+    match v with
+    | .lit (.strVal v) => .var v
+    | _ => .unk e
+  | Examples.Exp.binop e1 o e2 => .binop (reify e1) o (reify e2)
+  | Examples.Exp.rece f x e' =>
+    match f, x with
+    | .lit (.strVal f), .lit (.strVal x) => .rece f x (reify e')
+    | _, _ => .unk e'
+  | Examples.Exp.app e1 e2 => .app (reify e1) (reify e2)
+  | Examples.Exp.ife e1 e2 e3 => .ife (reify e1) (reify e2) (reify e3)
+  | _ => .unk e
+
+def subst (x : String) (v : Expr) (e : Exp) : Exp :=
+  match e with
+  | .val _ => e
+  | .var y => if x == y then .val v else e
+  | .binop e1 o e2 => .binop (subst x v e1) o (subst x v e2)
+  | .rece f y e' => .rece f y (if x == f || x == y then e' else subst x v e')
+  | .app e1 e2 => .app (subst x v e1) (subst x v e2)
+  | .ife e1 e2 e3 => .ife (subst x v e1) (subst x v e2)  (subst x v e3)
+  | .unk e => .unk (mkApp3 (mkConst ``Examples.subst) (mkStrLit x) v e)
+
+end Reify
+
+section
+open Lean Elab Tactic Meta Qq BI Std ProofMode
+@[irun_tac wpsubst _ _ _ _]
+def irunSubst : IRunTacticType := fun goal => do profileitM Exception "irunSubst" (← getOptions) do
+  let g ← instantiateMVars <| ← goal.getType
+  let some ig := parseIrisGoal? g | throwError "not in proof mode"
+  let { prop:=_, bi:=_, e:=_, hyps:=_, goal:=G } := ig
+
+  let .true := G.isAppOfArity ``wpsubst 5 | return none
+  -- TODO: Do something smarter here?
+  --let goals ← evalTacticAtRaw (← `(tactic | dsimp [wpsubst, subst])) goal
+  let .some x := Reify.rawStringLit? (G.getArg! 1) | return none
+  let v := G.getArg! 2
+  let P := G.getArg! 4
+  let e := Reify.reify (G.getArg! 3)
+  let e' := (Reify.subst x v e).unreify
+  let g' := {ig with goal := Expr.beta P #[e']}.toExpr
+--  let { ctx:=simpctx, simprocs, .. } ← mkSimpContext .missing (eraseLocal := false) (kind := .dsimp)
+--  let ⟨g', _⟩ ← Meta.dsimp g' simpctx simprocs
+  let goal' := ← goal.replaceTargetDefEq g'
+  --let goals ← evalTacticAtRaw (← `(tactic | try dsimp)) goal'
+
+
+--  let goals ← evalTacticAtRaw (← `(tactic | (conv => rhs; arg 0; unfold wpsubst) <;> dsimp [subst])) goal
+  --return .some (goals, [])
+  return .some ([goal'], [])
+
+@[irun_tac wpsimp _ _ _]
+def irunSimp : IRunTacticType := fun goal => do profileitM Exception "irunSimp" (← getOptions) do
+  let g ← instantiateMVars <| ← goal.getType
+  let some ig := parseIrisGoal? g | throwError "not in proof mode"
+  let { prop:=_, bi:=_, e:=_, hyps:=_, goal:=G } := ig
+
+  let .true := G.isAppOfArity ``wpsimp 6 | return none
+  -- TODO: Do something smarter here?
+  --let goals ← evalTacticAtRaw (← `(tactic | dsimp [wpsubst, subst])) goal
+  let n : Name ← reduceEval (G.getArg! 3)
+  let e := G.getArg! 4
+  let P := G.getArg! 5
+  let ext ← Lean.Meta.getSimpExtension? n
+  let theorems ← ext.get!.getTheorems
+  let { ctx:=simpctx, .. } ← goal.withContext <| mkSimpContext .missing (eraseLocal := false) (kind := .dsimp) (simpTheorems := pure theorems)
+  let ⟨e_new, _⟩ ← Meta.dsimp e simpctx {}
+  let g' := {ig with goal := Expr.beta P #[e_new]}.toExpr
+  let goal' := ← goal.replaceTargetDefEq g'
+  --let goals ← evalTacticAtRaw (← `(tactic | try dsimp)) goal'
+
+
+--  let goals ← evalTacticAtRaw (← `(tactic | (conv => rhs; arg 0; unfold wpsubst) <;> dsimp [subst])) goal
+  --return .some (goals, [])
+  return .some ([goal'], [])
+
+end
+end lang
+
+theorem exfalso {P : Prop} : P  :=
+  by sorry
+
+section
+variable {u} [BI.{u} PROP]
+
+theorem proof_intro_custom_auto (P G : PROP) :
+  ⊢ P -∗ G -∗ G ∗ True := by
+    istart
+    irun
+
+theorem proof_intro_pers_auto (P G : PROP) :
+  ⊢ P -∗ □ G -∗ G ∗ G ∗ True := by
+    istart
+    irun
+
+--set_option profiler true in
+#time theorem proof_intro_2 [BIAffine PROP] (P : Nat → PROP) :
+  ⊢ List.foldl (λ G n => iprop((P n) -∗ G)) (P 119) (List.range 120)
+:=
+  -- set_option trace.profiler true in by
+   by
+     dsimp [List.foldl, List.range, List.range.loop] <;> (repeat iintro _) <;> iassumption
+
+
+/-
+-- TODO: why does ilif sometimes take more than 1ms here if there a no lif in the goal?
+--set_option profiler true in
+--set_option profiler.threshold 1 in
+set_option maxRecDepth 30000 in
+#time theorem proof_cancel_2 (P : Nat → PROP) :
+  ⊢ List.foldl (λ G n => iprop((P n) -∗ G))
+    (List.foldl (λ G n => iprop(P n ∗ G)) iprop(True) (
+    -- List.reverse makes cancellation basically instant
+    -- List.reverse
+    (List.range 2)))
+    (List.range 2)
+:=
+  by
+    dsimp [List.foldl, List.range, List.range.loop, List.reverse]
+    istart
+    set_option trace.profiler true in
+    -- set_option trace.profiler.threshold 1 in
+    irun ∞
+-/
+
+theorem wp_test (P : Val -> PROP) :
+  P (.nat 10) ⊢ wp (Exp.binop (.val (.nat 5)) .plus (.val (.nat 5))) (λ v => iprop(P v ∗ True)) := by
+  istart
+  irun 1
+  irun 1
+  irun 1
+  irun 1
+  irun 1
+  irun 1
+  irun 1
+  irun 1
+  irun 1
+
+def rec_fn : Val :=
+  .recv "f" "x" (.ife (.binop (.var "x") .eq (.val (.nat 0))) (.val (.nat 0)) (.app (.var "f") (.binop (.var "x") .minus (.val (.nat 1)))))
+
+attribute [irun_simp] Nat.add_one_sub_one
+
+/-
+time for 200 iterations:
+- with match reduction, no dsimp in IRun, reified subst in irunSubst, solve if using trivial, wpsimp: ~1686ms
+- with match reduction, no dsimp in IRun, reified subst + dsimp in irunSubst, solve if using trivial: ~1723ms
+- with match reduction, no dsimp in IRun, reified subst in irunSubst, solve if using simp, wpsimp: ~2299ms
+- with match reduction, no dsimp in IRun, reified subst + dsimp in irunSubst, solve if using simp: ~2299ms
+- no match reduction, no dsimp in IRun, reified subst + dsimp in irunSubst, solve if using simp: ~2299ms
+- with match reduction, no dsimp in IRun, dsimp [wpsubst, subst] in irunSubst, solve if using simp: ~2991ms
+- dsimp in IRun, reified subst in irunSubst, solve if using simp: ~3725ms
+- dsimp in IRun, reified subst + dsimp in irunSubst, solve if using simp: ~3725ms
+
+comparison in Rocq:
+- 200 steps: 4579ms for rep liTStep, 5026ms for Qed
+- 100 steps: 1905ms for rep liTStep, 1496ms for Qed
+-/
+set_option profiler true in
+--set_option profiler.threshold 1 in
+#time theorem wp_test2 (P : Val -> PROP) :
+  P (.nat 0) ⊢ wp (.app (.val rec_fn) (.val (.nat 200))) (λ v => iprop(P v ∗ True)) := by
+  istart
+  unfold rec_fn
+  --isubst <;> iautoapply
+  --set_option trace.profiler true in
+  --set_option trace.profiler.threshold 1 in
+  --set_option diagnostics true in
+  --set_option profiler true in
+  irun ∞
+  -- rep 300 istep
+  --repeat' istep
+
+end
+
+end Iris.Examples
