src/Iris/Examples/Lithium.lean
@@ -1,0 +1,791 @@
+/-
+Copyright (c) 2025 Michael Sammler. All rights reserved.
+Released under Apache 2.0 license as described in the file LICENSE.
+Authors: Michael Sammler
+-/
+import Iris.BI
+import Iris.ProofMode
+import Iris.Examples.IRunAttr
+import Iris.Examples.IRun
+
+/-
+next steps:
+- rename tactics and everything to a consistent name
+- add support for ⌜P⌝ -∗ G
+- add support for ⌜P⌝ ∗ G
+- add support for lif where one cannot prove either side
+- add syntax for Lithium goals
+- look into performance
+- figure out how to avoid dsimp in wpsubst
+- define wp
+- add more lithium connectives
+- prove sorrys
+- do more examples
+- define a notation for the language
+- look into namespaces and using export
+-/
+
+syntax:min term " ≫ " term:min1 : term
+syntax:min term " ≫= " term:min1 : term
+
+macro_rules
+  | `($a ≫= $args) => `(.bind $a $args)
+  | `($a ≫ $args) => `(.bind $a λ _ => $args)
+
+namespace HBind
+class HBind (α : outParam (Type u)) (mα : Type v) (nβ : Type w) where
+  hbind : mα → (α → nβ) → nβ
+class HPure (α : outParam (Type u)) (mα : Type v) where
+  hpure : α → mα
+end HBind
+
+namespace Iris.Lithium
+open Lean BI Std HBind
+
+variable [BI.{u} PROP]
+
+structure Atom (α : Type v) where
+  ref : α → PROP
+
+structure InExM (α : Type v) where
+  body : α → PROP
+
+structure LithiumM (α : Type v) where
+  body : (α → PROP) → PROP
+  mono' E1 E2 : ⊢ body E1 -∗ (∀ a, E1 a -∗ E2 a) -∗ body E2
+
+namespace InExM
+
+variable {α : Type v} {β : Type w}
+
+def pure (a : α) : @InExM PROP α :=
+  InExM.mk λ b => iprop(⌜a = b⌝)
+
+def bind (L1 : @InExM PROP α) (L2 : α → @InExM PROP β) :
+  @InExM PROP β :=
+  InExM.mk λ b => iprop(∃ a, L1.body a ∗ (L2 a).body b)
+
+instance : Monad (@InExM PROP) where
+  pure := .pure
+  bind := .bind
+
+instance : HBind α (@InExM PROP α) (@InExM PROP β) where
+  hbind := .bind
+instance : HPure α (@InExM PROP α) where
+  hpure := .pure
+
+def atom (A : @Atom PROP α) : @InExM PROP α := InExM.mk A.ref
+def own (P : PROP) : @InExM PROP Unit := .mk λ _ => iprop(P)
+def ownP (P : PROP) : @InExM PROP PUnit := .mk λ _ => iprop(P)
+def prop (P : Prop) : @InExM PROP Unit := own iprop(⌜P⌝)
+def propP (P : Prop) : @InExM PROP PUnit := ownP iprop(⌜P⌝)
+
+end InExM
+
+namespace LithiumM
+
+variable {α : Type v} {β : Type w}
+
+def pure (a : α) : @LithiumM PROP _ α := {
+  body E := E a
+  mono' E1 E2 := by
+    dsimp
+    iintro HE Hwand
+    ispecialize Hwand HE
+    iassumption
+}
+
+def bind (G1 : @LithiumM PROP _ α) (G2 : α → @LithiumM PROP _ β) :
+  @LithiumM PROP _ β := {
+  body E := G1.body (λ a => (G2 a).body E)
+  mono' E1 E2 := by
+    dsimp
+    iintro HE Hwand
+    sorry
+}
+
+def bind2 (G1 : @LithiumM PROP _ α) (G2 : α → @LithiumM PROP _ β) :
+  @LithiumM PROP _ β := {
+  body E := G1.body (λ a => (G2 a).body E)
+  mono' E1 E2 := by
+    dsimp
+    iintro HE Hwand
+    sorry
+}
+
+instance : Monad (@LithiumM PROP _) where
+  pure := .pure
+  bind := .bind
+
+instance : HBind α (@LithiumM PROP _ α) (@LithiumM PROP _ β) where
+  hbind := .bind
+instance : HPure α (@LithiumM PROP _ α) where
+  hpure := .pure
+
+def exhale (L : @InExM PROP α) : @LithiumM PROP _ α := {
+  body E := iprop(∃ a, L.body a ∗ E a)
+  mono' E1 E2 := by
+    dsimp
+    iintro ⟨a, HL, HE⟩ Hwand
+    iexists a
+    isplit l [HL]
+    iassumption
+    ispecialize Hwand HE
+    iassumption
+}
+
+def inhale (L : @InExM PROP α) : @LithiumM PROP _ α := {
+  body E := iprop(∀ a, L.body a -∗ E a)
+  mono' E1 E2 := by
+    dsimp
+    iintro HE Hwand a HL
+    ispecialize HE HL
+    ispecialize Hwand HE
+    iassumption
+}
+
+def all (α : Type v) : @LithiumM PROP _ α := {
+  body E := iprop(∀ a, E a)
+  mono' E1 E2 := by
+    dsimp
+    iintro HE Hwand a
+    ispecialize HE a
+    ispecialize Hwand HE
+    iassumption
+}
+
+def done : @LithiumM PROP _ α := {
+  body E := iprop(True)
+  mono' E1 E2 := by
+    dsimp
+    iintro HE Hwand
+    iassumption
+}
+
+def lif (P : Prop) (G1 G2 : @LithiumM PROP _ α) : @LithiumM PROP _ α := {
+  body E := iprop((⌜P⌝ -∗ G1.body E) ∧ (⌜¬P⌝ -∗ G2.body E))
+  mono' E1 E2 := by
+    dsimp
+    iintro HE Hwand
+    sorry
+}
+
+def empty : Empty → PROP := λ e => nomatch e
+def emptyP : PEmpty → PROP := λ e => nomatch e
+
+def dualizing (G : @LithiumM PROP _ Empty) : @LithiumM PROP _ Unit := {
+  body E := iprop(G.body empty -∗ E ⟨⟩)
+  mono' E1 E2 := by
+    dsimp
+    iintro HE Hwand HG
+    ispecialize HE HG
+    ispecialize Hwand HE
+    iassumption
+}
+
+def dualizingP (G : @LithiumM PROP _ PEmpty) : @LithiumM PROP _ PUnit := {
+  body E := iprop(G.body emptyP -∗ E ⟨⟩)
+  mono' E1 E2 := by
+    dsimp
+    iintro HE Hwand HG
+    ispecialize HE HG
+    ispecialize Hwand HE
+    iassumption
+}
+
+def run (E : α → PROP) (G : @LithiumM PROP _ α) : PROP := G.body E
+-- TODO: What are good precedences?
+notation:35 G:36 " ⇓ " E:35 => run E G
+notation:35 G:36 " ⇓ " "!" => run empty G
+
+def entails (G1 G2 : @LithiumM PROP _ α) : Prop :=
+  ∀ E, G1.body E ⊢ G2.body E
+
+--notation:25 G1:29 ":-" G2:25 => (entails G2 G1)
+--set_option quotPrecheck false in -- TODO: Why is this necessary?
+--notation:25 G1:29 ":-" G2:25 => (∀ E, (G2 ⇓ E ⊢ G1 ⇓ E))
+notation:25 P:29 "⊣" Q:25 => (Q ⊢ P)
+
+--notation:25 G1:29 ":-" G2:25 => (run! G2 ⊢ run! G1)
+
+end LithiumM
+
+@[irun]
+theorem run_bind (G1 : @LithiumM PROP _ α) (G2 : α → LithiumM β)
+  (E : β → PROP) :
+   G1.bind G2 ⇓ E ⊣ (G1 ⇓ λ b => G2 b ⇓ E) := by
+    simp [LithiumM.bind, LithiumM.body, LithiumM.run]
+
+@[irun]
+theorem run_pure (a : α) (E : α → PROP) :
+   .pure a ⇓ E ⊣ E a := by
+    simp [LithiumM.pure, LithiumM.body, LithiumM.run]
+
+@[irun]
+theorem exhale_bind (L1 : @InExM PROP α) (L2 : α → InExM β) E :
+  .exhale (L1.bind L2) ⇓ E ⊣
+    LithiumM.exhale L1 ⇓ λ a => LithiumM.exhale (L2 a) ⇓ E := by
+    dsimp [bind, LithiumM.bind, LithiumM.exhale, LithiumM.body, InExM.bind, LithiumM.run]
+    sorry
+
+@[irun]
+theorem inhale_bind (L1 : @InExM PROP α) (L2 : α → InExM β) E :
+  .inhale (L1.bind L2) ⇓ E ⊣
+   LithiumM.inhale L1 ⇓ λ a => .inhale (L2 a) ⇓ E := by
+    dsimp [bind, LithiumM.bind, LithiumM.inhale, LithiumM.body, InExM.bind]
+    sorry
+
+@[irun]
+theorem exhale_pure (a : α) E :
+  .exhale (PROP:=PROP) (.pure a) ⇓ E ⊣ E a := by
+    dsimp [bind, LithiumM.pure, LithiumM.exhale, LithiumM.body, InExM.pure]
+    sorry
+
+@[irun]
+theorem inhale_pure (a : α) E :
+  .inhale (PROP:=PROP) (.pure a) ⇓ E ⊣ E a := by
+    dsimp [bind, LithiumM.pure, LithiumM.inhale, LithiumM.body, InExM.pure]
+    sorry
+
+
+def test_inexP (A : @Atom PROP (ULift.{u} Nat)) : @InExM PROP (ULift.{u} Bool) := do
+  let n ← .atom A
+  .ownP (A.ref n)
+  return ULift.up (n.down == 1)
+
+set_option pp.universes true
+
+def test_inex (A : @Atom PROP Nat) : @InExM PROP Bool :=
+  .atom A ≫= λ n =>
+  .own (A.ref n) ≫
+  .pure (n == 1)
+
+def test_inexh (A : @Atom PROP Nat) : @InExM PROP Bool :=
+  HBind.hbind (InExM.atom A) λ n =>
+  HBind.hbind (InExM.own (A.ref n)) λ _ =>
+  InExM.pure (n == 1)
+
+
+def test_lithiumP (A : @Atom PROP (ULift.{u} Nat)) : @LithiumM PROP _ (ULift.{u} Bool) := do
+  let b ← .exhale do
+    let n ← .atom A
+    return ULift.up (n.down == 1)
+  .inhale do
+    let n ← .atom A
+    .propP (b.down = (n.down == 1))
+    return ULift.up true
+
+
+def test_lithium (A : @Atom PROP Nat) : @LithiumM PROP _ Bool := do
+  (LithiumM.exhale <|
+    .atom A ≫= λ n =>
+    .pure (n == 1)) ≫= λ b =>
+  LithiumM.inhale <|
+    .atom A ≫= λ n =>
+    .prop (b = (n == 1)) ≫
+    .pure true
+
+-- set_option pp.universes true
+
+-- #check InExM.instHBind
+-- #check LithiumM.instHBind
+
+/--
+error: typeclass instance problem is stuck, it is often due to metavariables
+  HBind.{0, u, u} Bool (LithiumM.{u, 0} Bool) (LithiumM.{u, 0} Bool)
+-/
+#guard_msgs in
+def test_lithiumH (A : @Atom PROP Nat) : @LithiumM PROP _ Bool := do
+  HBind.hbind (LithiumM.exhale.{u} (α:=Bool) <|
+    HBind.hbind (InExM.atom A) λ n =>
+    HPure.hpure (n == 1)) λ b =>
+  LithiumM.inhale <|
+    HBind.hbind (InExM.atom A) λ n =>
+    HBind.hbind (InExM.prop (b = (n == 1))) λ _=>
+    HPure.hpure true
+
+end Iris.Lithium
+
+namespace Iris.ProofMode
+open Lean Elab Tactic Meta Qq BI Std Lithium
+
+theorem inhale_own_tac [BI PROP] {P A : PROP} (E : Unit → PROP)
+  (h : P ∗ A ⊢ E ())
+ : P ⊢ (LithiumM.inhale (.own A)) ⇓ E := by
+    simp [LithiumM.run, LithiumM.inhale, InExM.own, InExM.body]
+    sorry
+
+@[irun_tac (LithiumM.inhale (InExM.own _)) ⇓ _]
+def irunInhaleOwn : IRunTacticType := fun goal => do profileitM Exception "irunIntro" (← getOptions) do
+  let g ← instantiateMVars <| ← goal.getType
+  let some { prop, bi, e, hyps, goal:=G } := parseIrisGoal? g | throwError "not in proof mode"
+  let ~q(LithiumM.run $E (LithiumM.inhale (.own $A))) := G | return none
+  let ident ← `(binderIdent| _)
+  let (b, A') := if A.isAppOfArity ``intuitionistically 3 then
+      (q(true), A.getArg! 3)
+    else
+      (q(false), A)
+  let goals ← IO.mkRef #[]
+  let Q := q($E ())
+  let pf ← iCasesCore bi hyps Q b A A' ⟨⟩ (.one ident) fun hyps => do
+    let m ← mkFreshExprSyntheticOpaqueMVar <|
+      IrisGoal.toExpr { prop, bi, hyps, goal:=Q }
+    goals.modify (·.push m.mvarId!)
+    return m
+  let pf := q(@inhale_own_tac $prop $bi $e $A $E $pf)
+  goal.assign pf
+  return .some ((← goals.get).toList, [])
+
+theorem cancel [BI PROP] {p : Bool} {P P' A : PROP} {E}
+  (hP : P ⊣⊢ P' ∗ □?p A)
+  (h : P' ⊢ E ())
+ : P ⊢ LithiumM.exhale (.own A) ⇓ E := by
+   sorry
+   --hP.1.trans <| sep_comm.1.trans <| sep_mono intuitionisticallyIf_elim h
+
+@[irun_tac LithiumM.exhale (InExM.own _) ⇓ _]
+def irunCancel : IRunTacticType := fun goal => do profileitM Exception "irunCancel" (← getOptions) do
+  let g ← instantiateMVars <| ← goal.getType
+  let some { prop, bi, hyps, goal:=G } := parseIrisGoal? g | throwError "not in proof mode"
+  let ~q(LithiumM.exhale (.own $A) ⇓ $E) := G | return none
+  let some ⟨_inst, P', hyps, out, ty, b, _, pf⟩ ←
+    hyps.removeG false fun _ _ _ ty => do
+      -- logInfo m!"ty: ${ty}, A: ${A}"
+      if ← isDefEq ty A then return some ty else return none
+    | return none
+  have : $ty =Q $A := ⟨⟩
+  have : $out =Q iprop(□?$b $ty) := ⟨⟩
+  let m : Q($P' ⊢ $E ()) ← mkFreshExprSyntheticOpaqueMVar <|
+    IrisGoal.toExpr { prop, bi, hyps := hyps, goal := q($E ()) }
+  let pf := q(cancel $pf $m)
+  goal.assign pf
+  return .some ([m.mvarId!], [])
+
+theorem done_tac {α : Type _} [BI PROP] (P : PROP) (E : α → PROP)
+ : P ⊢ LithiumM.done ⇓ E := pure_intro .intro
+
+--set_option pp.universes true
+
+@[irun_tac LithiumM.done ⇓ _]
+def irunDone : IRunTacticType := fun goal => do profileitM Exception "irunTrue" (← getOptions) do
+  let g ← instantiateMVars <| ← goal.getType
+  let some { prop:=prop, bi:=bi, hyps:=_, e, goal:=G } := parseIrisGoal? g | throwError "not in proof mode"
+  match_expr G with
+  | LithiumM.run _ _ α E G =>
+    let .true := G.isAppOfArity ``LithiumM.done 3 | return none
+    let pf := mkApp5 (.const ``done_tac G.getAppFn.constLevels!) prop α bi e E
+    goal.assign pf
+    return .some ([], [])
+  | _ => return none
+
+
+theorem lif_true {α : Type _} [BI PROP] {cond} {P : PROP} (G1 : LithiumM α) G2 E
+  (h1 : cond)
+  (h2 : P ⊢ G1 ⇓ E)
+ : P ⊢ .lif cond G1 G2 ⇓ E :=
+   sorry
+
+theorem lif_false {α : Type _} [BI PROP] {cond} {P : PROP} (G1 : LithiumM α) G2 E
+  (h1 : ¬ cond)
+  (h2 : P ⊢ G2 ⇓ E)
+ : P ⊢ .lif cond G1 G2 ⇓ E :=
+   sorry
+
+syntax "istepsolve" : tactic
+--macro_rules
+--  | `(tactic|istepsolve) => `(tactic|trivial)
+macro_rules
+  | `(tactic|istepsolve) => `(tactic|solve| simp)
+
+@[irun_tac LithiumM.lif _ _ _ ⇓ _]
+def irunLif : IRunTacticType := fun goal => do profileitM Exception "irunLif" (← getOptions) do
+  let g ← instantiateMVars <| ← goal.getType
+  let some { prop, bi, e, hyps, goal:=G } := parseIrisGoal? g | throwError "not in proof mode"
+  let ~q(LithiumM.lif $cond $G1 $G2 ⇓ $E) := G | return none
+
+  let mcond : Q($cond) ← mkFreshExprSyntheticOpaqueMVar cond
+  try
+    let _ ← evalTacticAtRaw (← `(tactic|istepsolve)) mcond.mvarId!
+    let m : Q($e ⊢ $G1 ⇓ $E) ← mkFreshExprSyntheticOpaqueMVar <|
+      IrisGoal.toExpr { prop, bi, hyps := hyps, goal := q($G1 ⇓ $E) }
+    let pf := q(lif_true $G1 $G2 $E $mcond $m)
+    goal.assign pf
+    return .some ([m.mvarId!], [])
+  catch _ => pure ()
+
+  let mnegcond : Q(¬$cond) ← mkFreshExprSyntheticOpaqueMVar q(¬ $cond)
+  try
+    let _ ← evalTacticAt (← `(tactic|istepsolve)) mnegcond.mvarId!
+    let m : Q($e ⊢ $G2 ⇓ $E) ← mkFreshExprSyntheticOpaqueMVar <|
+      IrisGoal.toExpr { prop, bi, hyps := hyps, goal := q($G2 ⇓ $E) }
+    let pf := q(lif_false $G1 $G2 $E $mnegcond $m)
+    goal.assign pf
+    return .some ([m.mvarId!], [])
+  catch _ => pure ()
+
+  throwError "Cannot solve either side of lif"
+
+section test
+variable {u} [BI.{u} PROP]
+
+theorem test1 (P : Nat → PROP) (Q : PROP) :
+  ⊢ (.inhale (.own Q) ≫
+      .inhale (.own (P 1)) ≫
+      .inhale (.own (P 2)) ≫
+      .inhale (.own iprop(⌜1 = 1⌝)) ≫
+      .exhale (.own (P 1) ≫ .own (P 2)) ≫
+      .exhale (.own Q) ≫
+   .done) ⇓ ! := by
+     istart
+     irun ∞
+
+
+theorem test_intro_cancel (P G : PROP) :
+  ⊢ .inhale (.own P ≫ .own G) ⇓ λ _ =>
+     .exhale (.own G) ⇓ λ _ =>
+     .done ⇓ ! := by
+    istart
+    irun 1
+    irun 1
+    irun 1
+    irun 1
+    irun 1
+
+/-
+--set_option profiler true in
+--set_option profiler.threshold 1 in
+set_option maxRecDepth 30000 in
+#time theorem proof_cancel_2 (P : Nat → PROP) :
+  ⊢ (List.foldl (λ G n => LithiumM.bind (.inhale (.own (P n))) λ _ => G)
+    (List.foldl (λ G n => LithiumM.bind (.exhale (.own (P n))) λ _ => G) .done (
+    -- List.reverse makes cancellation basically instant
+    -- List.reverse
+    (List.range 2)))
+    (List.range 2)) ⇓ !
+:=
+  by
+    dsimp [List.foldl, List.range, List.range.loop, List.reverse]
+    istart
+    -- set_option trace.profiler true in
+    -- set_option trace.profiler.threshold 1 in
+    irun ∞
+
+--set_option profiler true in
+--set_option profiler.threshold 1 in
+set_option maxRecDepth 30000 in
+#time theorem proof_cancel_3 (P : Nat → PROP) :
+  ⊢ (List.foldl (λ G n => LithiumM.inhale (.own (P n)) ⇓ λ _ => G)
+    (List.foldl (λ G n => LithiumM.exhale (.own (P n)) ⇓ λ _ => G)
+      (.done ⇓ !) (
+    -- List.reverse makes cancellation basically instant
+    -- List.reverse
+    (List.range 100)))
+    (List.range 100))
+:=
+  by
+    dsimp [List.foldl, List.range, List.range.loop, List.reverse]
+    istart
+    -- set_option trace.profiler true in
+    -- set_option trace.profiler.threshold 1 in
+    -- irun ∞
+    sorry
+-/
+
+end test
+
+end Iris.ProofMode
+
+namespace Iris.Examples
+open Lithium
+
+section lang
+variable {u} [BI.{u} PROP]
+def Loc : Type := Nat
+
+inductive Binop where
+| plus | minus | eq
+
+mutual
+inductive Val where
+| nat : Nat -> Val
+| loc : Loc -> Val
+| recv : String -> String -> Exp -> Val
+inductive Exp where
+| val : Val -> Exp
+| var : String -> Exp
+| binop : Exp -> Binop -> Exp -> Exp
+| rece : String -> String -> Exp -> Exp
+| app : Exp -> Exp -> Exp
+| ife : Exp -> Exp -> Exp -> Exp
+end
+
+def subst (x : String) (v : Val) (e : Exp) : Exp :=
+  match e with
+  | .val _ => e
+  | .var y => if x == y then .val v else e
+  | .binop e1 o e2 => .binop (subst x v e1) o (subst x v e2)
+  | .rece f y e' => .rece f y (if x == f || x == y then e' else subst x v e')
+  | .app e1 e2 => .app (subst x v e1) (subst x v e2)
+  | .ife e1 e2 e3 => .ife (subst x v e1) (subst x v e2)  (subst x v e3)
+
+def wp [BI PROP] (e : Exp) (P : Val -> PROP) : PROP := by sorry
+
+theorem wp_wand e (P1 P2 : Val -> PROP) :
+  ⊢ wp e P1 -∗ (∀ v, P1 v -∗ P2 v) -∗ wp e P2
+  := by sorry
+
+
+/- Proof automation begins here -/
+
+def expr_ok (e : Exp) : @LithiumM PROP _ Val := {
+  body := wp e
+  mono' := wp_wand e
+}
+
+def expr_okP (e : Exp) : @LithiumM PROP _ (ULift.{u} Val) := {
+  body E := wp e (λ v => E (ULift.up v))
+  mono' := by sorry
+}
+
+/- problem: Monad is not fully universe polymorphic -/
+def fn_specP (v : Val) (G : Val → @LithiumM PROP _ (Val → @LithiumM PROP _ PEmpty)) : PROP :=
+  iprop(∀ (E : ULift.{u} Val → PROP) va,
+  (LithiumM.run E do
+    let L' : Val → LithiumM PEmpty ← G va
+    let vr ← .all (ULift.{u} Val)
+    LithiumM.dualizingP (L' vr.down)
+    return vr)
+  -∗
+  wp (.app (.val v) (.val va)) λ v => E (ULift.up v))
+
+-- set_option pp.universes true
+
+def fn_spec (v : Val) (G : Val → @LithiumM PROP _ (Val → @LithiumM PROP _ Empty)) : PROP :=
+  iprop(∀ E va,
+  (.bind (G va) λ L' =>
+   .bind (.all Val) λ vr =>
+   .bind (.dualizing (L' vr)) λ _ =>
+   .pure vr) ⇓ E
+  -∗
+  wp (.app (.val v) (.val va)) E)
+
+def nat_ok (v : Val) : @LithiumM PROP _ Nat := {
+  body E := iprop(∃ n, ⌜v = .nat n⌝ ∗ E n)
+  mono' E1 E2 := by sorry
+}
+
+def recv_ok (v : Val) : @LithiumM PROP _ (String × String × Exp) := {
+  body E := iprop(∃ f x e, ⌜v = .recv f x e⌝ ∗ E (f, x, e))
+  mono' E1 E2 := by sorry
+}
+
+def subst_ok (x : String) (v : Val) (e : Exp) : @LithiumM PROP _ Exp := {
+  body E := E (subst x v e)
+  mono' E1 E2 := by
+    simp
+    sorry
+}
+
+@[irun]
+theorem nat_ok_nat (n : Nat) (E : Nat → PROP) :
+  nat_ok (.nat n) ⇓ E ⊣ E n := by
+  dsimp [nat_ok, LithiumM.run, LithiumM.body]
+  iintro HP
+  iexists _
+  isplit
+  · ipure_intro
+    rfl
+  · iassumption
+
+@[irun]
+theorem recv_ok_rec f x e (E : (String × String × Exp) -> PROP) :
+  recv_ok (.recv f x e) ⇓ E ⊣ E (f, x, e) := by
+  dsimp [recv_ok, LithiumM.run, LithiumM.body]
+  iintro HP
+  iexists _
+  iexists _
+  iexists _
+  isplit
+  · ipure_intro
+    rfl
+  · iassumption
+
+@[irun]
+theorem expr_ok_val v (E : Val -> PROP) :
+  expr_ok (.val v) ⇓ E ⊣ E v := by sorry
+
+@[irun]
+theorem expr_ok_plus e1 e2 (E : Val -> PROP) :
+  expr_ok (Exp.binop e1 .plus e2) ⇓ E ⊣
+   expr_ok e1 ⇓ λ v1 =>
+   expr_ok e2 ⇓ λ v2 =>
+   nat_ok v1 ⇓ λ n1 =>
+   nat_ok v2 ⇓ λ n2 => E (.nat (n1 + n2)) := by sorry
+
+@[irun]
+theorem expr_ok_minus e1 e2 (E : Val -> PROP) :
+  expr_ok (Exp.binop e1 .minus e2) ⇓ E ⊣
+   expr_ok e1 ⇓ λ v1 =>
+   expr_ok e2 ⇓ λ v2 =>
+   nat_ok v1 ⇓ λ n1 =>
+   nat_ok v2 ⇓ λ n2 => E (.nat (n1 - n2)) := by sorry
+
+@[irun]
+theorem expr_ok_eq e1 e2 (E : Val -> PROP) :
+  expr_ok (Exp.binop e1 .eq e2) ⇓ E ⊣
+   expr_ok e1 ⇓ λ v1 =>
+   expr_ok e2 ⇓ λ v2 =>
+   nat_ok v1 ⇓ λ n1 =>
+   nat_ok v2 ⇓ λ n2 => E (.nat (if n1 == n2 then 1 else 0)) := by sorry
+
+@[irun]
+theorem expr_ok_rec f x e (E : Val -> PROP) :
+  expr_ok (.rece f x e) ⇓ E ⊣ E (.recv f x e) := by sorry
+
+@[irun]
+theorem expr_ok_app e1 e2 (E : Val -> PROP) :
+  expr_ok (.app e1 e2) ⇓ E ⊣
+   expr_ok e2 ⇓ λ v2 =>
+   expr_ok e1 ⇓ λ v1 =>
+   recv_ok v1 ⇓ λ ⟨f, x, e'⟩ =>
+   subst_ok x v2 e' ⇓ λ e =>
+   subst_ok f (.recv f x e') e ⇓ λ e =>
+   expr_ok e ⇓ E := by sorry
+
+@[irun]
+theorem expr_ok_if e1 e2 e3 (E : Val -> PROP) :
+  (expr_ok e1 ⇓ λ v1 =>
+   nat_ok v1 ⇓ λ n1 =>
+   LithiumM.lif (n1 ≠ 0) (expr_ok e2) (expr_ok e3) ⇓ E) ⊢
+  expr_ok (.ife e1 e2 e3) ⇓ E := by sorry
+
+namespace Reify
+open Lean
+inductive Exp where
+| val : Expr -> Exp -- we do not need to reify values
+| var : String -> Exp
+| binop : Exp -> Expr -> Exp -> Exp
+| rece : String -> String -> Exp -> Exp
+| app : Exp -> Exp -> Exp
+| ife : Exp -> Exp -> Exp -> Exp
+| unk : Expr -> Exp
+deriving Inhabited, Repr
+
+-- should this be ToExpr?
+def Exp.unreify : Exp → Expr
+  | .val v => mkApp (mkConst ``Examples.Exp.val) v
+  | .var v => mkApp (mkConst ``Examples.Exp.var) (mkStrLit v)
+  | .binop e1 o e2 => mkApp3 (mkConst ``Examples.Exp.binop) (unreify e1) o (unreify e2)
+  | .rece f x e => mkApp3 (mkConst ``Examples.Exp.rece) (mkStrLit f) (mkStrLit x) (unreify e)
+  | .app e1 e2 => mkApp2 (mkConst ``Examples.Exp.app) (unreify e1) (unreify e2)
+  | .ife e1 e2 e3 => mkApp3 (mkConst ``Examples.Exp.ife) (unreify e1) (unreify e2) (unreify e3)
+  | .unk e => e
+
+
+def rawStringLit? : Expr → Option String
+  | .lit (.strVal v) => .some v
+  | _ => .none
+
+
+partial def reify (e : Expr) : Exp :=
+  match_expr e with
+  | Examples.Exp.val v => .val v
+  | Examples.Exp.var v =>
+    match v with
+    | .lit (.strVal v) => .var v
+    | _ => .unk e
+  | Examples.Exp.binop e1 o e2 => .binop (reify e1) o (reify e2)
+  | Examples.Exp.rece f x e' =>
+    match f, x with
+    | .lit (.strVal f), .lit (.strVal x) => .rece f x (reify e')
+    | _, _ => .unk e'
+  | Examples.Exp.app e1 e2 => .app (reify e1) (reify e2)
+  | Examples.Exp.ife e1 e2 e3 => .ife (reify e1) (reify e2) (reify e3)
+  | _ => .unk e
+
+def subst (x : String) (v : Expr) (e : Exp) : Exp :=
+  match e with
+  | .val _ => e
+  | .var y => if x = y then .val v else e
+  | .binop e1 o e2 => .binop (subst x v e1) o (subst x v e2)
+  | .rece f y e' => .rece f y (if x == f || x == y then e' else subst x v e')
+  | .app e1 e2 => .app (subst x v e1) (subst x v e2)
+  | .ife e1 e2 e3 => .ife (subst x v e1) (subst x v e2)  (subst x v e3)
+  | .unk e => .unk (mkApp3 (mkConst ``Examples.subst) (mkStrLit x) v e)
+
+end Reify
+
+section
+open Lean Elab Tactic Meta Qq BI Std ProofMode
+@[irun_tac subst_ok _ _ _ ⇓  _]
+def irunSubst : IRunTacticType := fun goal => do profileitM Exception "irunSubst" (← getOptions) do
+  let g ← instantiateMVars <| ← goal.getType
+  let some ig := parseIrisGoal? g | throwError "not in proof mode"
+  let { prop:=_, bi:=_, e:=_, hyps:=_, goal:=G } := ig
+
+  let .true := G.isAppOfArity ``LithiumM.run 5 | return none
+  let E := G.getArg! 3
+  let G' := G.getArg! 4
+  let .true := G'.isAppOfArity ``subst_ok 5 | return none
+  let .some x := Reify.rawStringLit? (G'.getArg! 2) | return none
+  let v := G'.getArg! 3
+  let e := Reify.reify (G'.getArg! 4)
+  let e' := (Reify.subst x v e).unreify
+--  let e' ← whnfR (mkApp3 (mkConst ``subst) (G'.getArg! 2) (G'.getArg! 3) (G'.getArg! 4))
+--  logInfo m!"{repr e}"
+--  logInfo m!"{e'}"
+  -- TODO: Do something smarter here?
+  let g' := {ig with goal := Expr.beta E #[e']}.toExpr
+  let { ctx:=simpctx, simprocs, .. } ← mkSimpContext .missing (eraseLocal := false) (kind := .dsimp)
+  let ⟨g', _⟩ ← Meta.dsimp g' simpctx simprocs
+  let goal' := ← goal.replaceTargetDefEq g'
+  -- let goals ← evalTacticAtRaw (← `(tactic | (conv => rhs; arg 0; unfold LithiumM.run) <;> (conv => rhs; arg 1; unfold subst_ok) <;> dsimp [LithiumM.body, subst])) goal
+--  let goals ← evalTacticAtRaw (← `(tactic | dsimp [LithiumM.run, subst_ok, subst])) goal
+  -- let goals ← evalTacticAtRaw (← `(tactic | try dsimp)) goal'
+  return .some ([goal'], [])
+  -- return .some (goals, [])
+
+end
+end lang
+
+section
+variable {u} [BI.{u} PROP]
+
+theorem expr_ok_test (P : Val -> PROP) :
+  ⊢ .inhale (.own (P (.nat 10))) ⇓ λ _ =>
+     expr_ok (.binop (.val (.nat 5)) .plus (.val (.nat 5))) ⇓ λ v =>
+     .exhale (.own (P v)) ⇓ λ _ =>
+     .done ⇓ ! := by
+  istart
+  irun 1
+  irun 1
+  irun 1
+  irun 1
+  irun 1
+  irun 1
+  irun 1
+  irun 1
+
+def rec_fn : Val :=
+  .recv "f" "x" (.ife (.binop (.var "x") .eq (.val (.nat 0))) (.val (.nat 0)) (.app (.var "f") (.binop (.var "x") .minus (.val (.nat 1)))))
+
+attribute [irun_simp] Nat.add_one_sub_one
+
+set_option profiler true in
+--set_option profiler.threshold 1 in
+#time theorem expr_ok_test2 (P : Val -> PROP) :
+   ⊢ .inhale (.own (P (.nat 0))) ⇓ λ _ =>
+      expr_ok (.app (.val rec_fn) (.val (.nat 200))) ⇓ λ v =>
+      .exhale (.own (P v)) ⇓ λ _ =>
+      .done ⇓ ! := by
+  istart
+  unfold rec_fn
+  --isubst <;> iautoapply
+  --set_option trace.profiler true in
+  --set_option trace.profiler.threshold 1 in
+  --set_option diagnostics true in
+  --set_option profiler true in
+  irun ∞
+
+end
+end Iris.Examples
